checked: bless proofs

src/Pipit.Exp.Checked.Base.fst
@@ -50,16 +50,16 @@ let rec check (#t: table u#i u#j) (#c: context t) (#a: t.ty)
       bigstep_always rows rely) /\
     // Check rely subexpression
     check mode rows rely /\
-    // Contract definition:
-    (forall (vs: list (t.ty_sem a) { bigsteps_prop rows body vs}).
-      // Check that if rely is trues, then guarantee is trues.
-      (PM.prop_status_contains mode PM.PSValid ==>
-        bigstep_always rows rely ==>
-        bigstep_always (CR.extend1 vs rows) guar) /\
-      // If rely is trues, then also check sub-properties of body and guar
-      (bigstep_always rows rely ==>
-        (check mode rows body /\
-        check mode (CR.extend1 vs rows) guar)))
+    // Contract definition assumes rely is trues:
+    (bigstep_always rows rely ==>
+      (forall (vs: list (t.ty_sem a) { bigsteps_prop rows body vs}).
+        // If rely and we are in contract-check-definition mode, then guarantee is trues
+        (PM.prop_status_contains mode PM.PSValid ==>
+          bigstep_always (CR.extend1 vs rows) guar) /\
+        // If rely is trues and any mode, then check sub-properties of guar
+        check mode (CR.extend1 vs rows) guar) /\
+      // If rely is trues and any mode, then check sub-properties of body
+      check mode rows body)
 
 and check_apps (#t: table) (#c: context t) (#a: funty t.ty)
   (mode: PM.check_mode)
